Checkpoint control flow proof principles

src/goose_lang/lib/loop/impl.v
@@ -1,37 +1,51 @@
-From Perennial.goose_lang Require Import lang notation.
+From Perennial.goose_lang Require Import lang notation exception.
 
 Section goose_lang.
 Context {ext: ffi_syntax}.
 
-(* idiomatic wrappers for loop control flow *)
-Definition Continue: val := #true.
-Definition Break: val := #false.
+Definition do_break : val := λ: "v", (#(str "break"), Var "v").
+Definition do_continue : val := λ: "v", (#(str "continue"), Var "v").
 
-Definition For: val :=
+Definition break_val : val := (#(str "break"), #()).
+Definition continue_val : val := (#(str "continue"), #()).
+Definition execute_val : val := (#(str "execute"), #()).
+
+Definition do_for: val :=
   λ: "cond" "body" "post",
-  (rec: "loop" <> :=
-     let: "continue" :=
-        (if: (Var "cond") #()
-         then (Var "body") #()
-         else #false) in
-     if: (Var "continue")
-     then (Var "post") #();; (Var "loop") #()
-     else #()) #().
+  (rec: "loop" <> := exception_do (
+   if: ~(Var "cond") #() then (return: #())
+   else
+     let: "b" := (Var "body") #() in
+     if: Fst $ Var "b" = #(str "break") then (return: (do: #())) else (do: #()) ;;;
+     if: (Fst $ Var "b" = #(str "continue")) || (Fst $ Var "b" = #(str "execute"))
+          then (do: (Var "post") #();;; return: (Var "loop") #()) else do: #() ;;;
+     return: Var "b"
+  )) #().
 
-Definition Loop: val :=
+Definition do_loop: val :=
   λ: "body",
-  (rec: "loop" <> :=
-     let: "continue" := (Var "body") #() in
-     if: Var "continue"
-     then (Var "loop") #()
-     else #()) #().
+  (rec: "loop" <> := exception_do (
+     let: "b" := (Var "body") #() in
+     if: Fst $ Var "b" = #(str "break") then (return: (do: #())) else (do: #()) ;;;
+     if: (Fst $ Var "b" = #(str "continue")) || (Fst $ Var "b" = #(str "execute"))
+          then (return: (Var "loop") #()) else do: #() ;;;
+     return: Var "b"
+  )) #().
 
 End goose_lang.
 
-Notation "'for:' cond ; post := e" := (For cond%E e%E post%E)
+Global Notation "break: e" := (do_break e%E)
+  (at level 90, e at level 85,
+      format "break:  '[' e ']'") : expr_scope.
+
+Global Notation "continue: e" := (do_continue e%E)
+  (at level 90, e at level 85,
+      format "continue:  '[' e ']'") : expr_scope.
+
+Notation "'for:' cond ; post := e" := (do_for cond%E e%E post%E)
   (at level 200, cond, post at level 1, e at level 200,
    format "'[' 'for:'  cond  ;  post  :=  '/  ' e ']'") : expr_scope.
 
-Notation "'for:' := e" := (Loop (LamV BAnon e%E))
+Notation "'for:' := e" := (do_loop (LamV BAnon e%E))
   (at level 200, e at level 200,
    format "'[' 'for:'  :=  '/  ' e ']'") : expr_scope.
